Start temporal logic

src/tlogic/LogicSyntaxHOAS.v
@@ -3,7 +3,6 @@ From sflib Require Import sflib.
 From Fairness Require Import PCM IProp IPM IndexedInvariants.
 From iris Require Import bi.big_op.
 From iris Require base_logic.lib.invariants.
-Require Import Program.
 
 Module Syntax.
 
@@ -16,7 +15,35 @@ Module Syntax.
     Inductive type : Type :=
     | baseT (t : T) : type
     | formulaT : type
-    | arrowT : type -> type -> type.
+    | prodT : type -> type -> type
+    | sumT : type -> type -> type
+    | listT : type -> type
+    | funT : type -> type -> type
+    | gmapTpos : type -> type.
+    (* | gmapT (K : Type) {EqDec : EqDecision K} {Cnt : Countable K} : type -> type. *)
+
+  (* If we define for a general gmapT with EqDec and Countable,
+      universe inconsistency when checking (in TemporalLogic.Atoms)
+      ==========    
+      Context `{Σ : GRA.t}.
+      Context `{T : Type}.
+      Context `{TSem : T -> Type}.
+      Local Notation typing := (@Syntax.Typ T TSem (@t T)).
+      Local Notation As := (fun (i : index) => @t T (typing i)).
+
+      Context `{@GRA.inG (IInvSetRA As) Σ}.
+      ==========    
+      with an error message
+      ==========    
+      The term "t" has type
+      "Type@{max(Set+1,Fairness.LogicSyntaxHOAS.59,Syntax.type.u0+1,Fairness.LogicSyntaxHOAS.64,Fairness.LogicSyntaxHOAS.65,RelDecision.u0,RelDecision.u1)}"
+      while it is expected to have type "Type@{IInvSetRA.u0}" (universe inconsistency: Cannot enforce
+      Fairness.LogicSyntaxHOAS.64 <= IInvSetRA.u0 because IInvSetRA.u0 <= InvSetRA.u0
+      <= URA.agree_obligation_4.u0 <= URA.t.u0 < MRet.u0 = Fairness.LogicSyntaxHOAS.64).
+      ==========    
+      Seems like there is a strict order between URA.t and MRet,
+      and either EqDec or Countable uses MRet.
+   *)
 
   End TYPE.
 
@@ -55,7 +82,12 @@ Module Syntax.
       match ty with
       | baseT b => TSem b
       | formulaT => unit
-      | arrowT t1 t2 => (Typ_0 t1 -> Typ_0 t2)
+      | prodT ty1 ty2 => prod (Typ_0 ty1) (Typ_0 ty2)
+      | sumT ty1 ty2 => sum (Typ_0 ty1) (Typ_0 ty2)
+      | listT ty' => list (Typ_0 ty')
+      | funT ty1 ty2 => (Typ_0 ty1 -> Typ_0 ty2)
+      | gmapTpos ty' => gmap positive (Typ_0 ty')
+      (* | @gmapT _ K EqDec Cnt ty' => @gmap K EqDec Cnt (Typ_0 ty') *)
       end.
 
     Fixpoint Typ (i : index) : @type T -> Type :=
@@ -66,70 +98,16 @@ Module Syntax.
         match ty with
         | baseT b => TSem b
         | formulaT => @t T (Typ j) (As (Typ j))
-        | arrowT t1 t2 => (Typ_aux t1 -> Typ_aux t2)
+        | prodT ty1 ty2 => prod (Typ_aux ty1) (Typ_aux ty2)
+        | sumT ty1 ty2 => sum (Typ_aux ty1) (Typ_aux ty2)
+        | listT ty' => list (Typ_aux ty')
+        | funT ty1 ty2 => (Typ_aux ty1 -> Typ_aux ty2)
+        | gmapTpos ty' => gmap positive (Typ_aux ty')
+        (* | @gmapT _ K EqDec Cnt ty' => @gmap K EqDec Cnt (Typ_aux ty') *)
         end
       end.
 
   End INTERP_TYPE.
-
-  Section TEST.
-
-    Context `{T : Type}.
-    Context `{TSem : T -> Type}.
-
-    (* Atoms should not interpret arguments. *)
-    Inductive As (V : @type T -> Type) : Type :=
-      | owni (p : V formulaT)
-    .
-    (* Inductive As (V : @type T -> Type) : Type := *)
-    (*   | owni (i : index) (p : @t T V (As V)) *)
-    (* . *)
-
-    Definition typing (i : index) : @type T -> Type :=
-      @Typ T TSem As i.
-
-    (* Definition ttt1 : As (typing 2) := owni (typing 2) 0 (ex formulaT (fun s => pure (s = empty))). *)
-    (* Compute ttt1. *)
-    Definition ttt1 : As (typing 2) := owni (typing 2) (ex formulaT (fun s => pure (s = empty))).
-    Compute ttt1.
-    Goal typing 2 formulaT = @t T (typing 1) (As (typing 1)).
-    Proof.
-      ss.
-    Qed.
-
-    Definition inv (i : index) (p : typing i formulaT) :
-      @t T (typing i) (As (typing i)) :=
-      atom (owni _ p).
-    (* Definition inv (n i : index) (p : @t T (typing i) (As (typing i))) : *)
-    (*   @t T (typing i) (As (typing i)) := *)
-    (*   atom (owni _ n p). *)
-    Definition wsat (i : index) :
-      @t T (typing i) (As (typing i)) :=
-      ex formulaT (fun (p : typing i formulaT) => sepconj (lift p) (inv i p)).
-
-    (* Definition inv0 (n i : index) (p : @t T (typing 2) (As (typing 2))) : *)
-    (*   @t T (typing 3) (As (typing 2)) := *)
-    (*   atom (owni _ n p). *)
-
-    (* (* Definition of As enforces that  *)
-    (*    p should have the same typing level for itself and its atom  *)
-    (*  *) *)
-    (* Fail Definition inv1 (n : index) (p : @t T (typing 2) (As (typing 3))) : *)
-    (*   @t T (typing 2) (As (typing 3)) := *)
-    (*   atom (owni _ n p). *)
-
-    (* Definition inv2 q := *)
-    (*   inv 0 3 (atom (owni _ 1 (atom (owni _ 2 q)))). *)
-
-    (* Fail Definition inv2' q := *)
-    (*   inv 0 3 (atom (owni _ 1 (atom (owni (typing 2) 2 q)))). *)
-
-    (* Set Printing All. *)
-
-    (* Definition inv (N : namespace) P := *)
-    (*   (∃ p, ∃ i, ⌜prop p = P⌝ ∧ ⌜i ∈ (↑N : coPset)⌝ ∧ OwnI n i p)%I. *)
-
-  End TEST.
 
   Section INTERP.
 
@@ -198,435 +176,30 @@ Module Syntax.
 
     Context `{Atoms : @IInvSet Σ (fun (n : index) => As (typing n))}.
 
-    Global Instance IIS : @IInvSet Σ Formulas :=
+    Global Instance IISet : @IInvSet Σ Formulas :=
       {| prop := @to_semantics Σ T TSem As Atoms |}.
 
   End INDEXED_INVSET.
 
-  TODO
+  Section INV_IN.
 
-  Section TEST.
+    Context `{Σ : GRA.t}.
+    Context `{T : Type}.
+    Context `{TSem : T -> Type}.
+    Context `{As : (@type T -> Type) -> Type}.
 
-    Context `{A : Type}.
+    Local Notation typing := (@Typ T TSem As).
+    Local Notation Formulas := (fun (i : index) => @t T (typing i) (As (typing i))).
 
-    Variant tBase := | tBool | tNat.
-    Definition tBase_sem (b : tBase) : Type :=
-      match b with | tBool => bool | tNat => nat end.
+    Context `{Atoms : @IInvSet Σ (fun (n : index) => As (typing n))}.
 
-    Let Var := @Var tBase tBase_sem A.
+    Global Program Instance IIIn (i : index) (p : Formulas i)
+      : @IInvIn Σ Formulas IISet i (@to_semantics Σ T TSem As Atoms i p) :=
+      { inhabitant := p }.
+    Next Obligation.
+      intros. simpl in *. done.
+    Qed.
 
-    Compute Var 3 formulaT.
-
-    (* Goal Var 3 formulaT = @t _ (Var 2) A formulaT. *)
-    Goal Var 3 formulaT = @t _ (Var 2) A.
-    Proof. ss. Qed.
-
-    Definition syn_bad i := @t tBase (@Var i) A.
-    Notation syn i := (@t tBase (@Var i) A).
-
-    (* Definition form1 : @syn 2 formulaT := *)
-    Definition form1 : @syn 2 :=
-      @ex _ _ _ (baseT tBool) (fun b => empty).
-
-    (* Goal (syn 1 formulaT) = (Var 2 formulaT). *)
-    Goal (syn 1) = (Var 2 formulaT).
-    Proof. ss. Qed.
-
-    (* Definition form2 : @syn 2 formulaT := *)
-      (* @ex _ _ _ formulaT (fun (s : Var 2 formulaT) => and (var _ s) (var _ s)). *)
-    Definition form2 : @syn 2 :=
-      @ex _ _ _ formulaT (fun (s : Var 2 formulaT) => pure (s = impl empty empty)).
-
-    (* Definition form3 : @syn 2 formulaT := *)
-    (*   @ex _ _ _ formulaT (fun (s : @t tBase (Var 1) A formulaT) => and (var _ s) (var _ s)). *)
-    Definition form3 : @syn 2 :=
-      @ex _ _ _ formulaT (fun (s : @t tBase (Var 1) A) => pure (s = impl empty empty)).
-
-    (* Definition form4 : @syn 2 formulaT := *)
-    (*   @ex _ _ _ formulaT (fun (s : @syn 1 formulaT) => and (var _ s) (var _ s)). *)
-    Definition form4 : @syn 2 :=
-      @ex _ _ _ formulaT (fun (s : @syn 1) => pure (s = impl empty empty)).
-
-    (* Definition form5 : @syn 2 formulaT := *)
-    (*   @ex _ _ _ formulaT (fun (s : @syn 1 formulaT) => pure (s = wand empty empty)). *)
-    Definition form5 : @syn 2 :=
-      @ex _ _ _ formulaT (fun (s : @syn 1) => pure (s = wand empty empty)).
-
-  End TEST.
+  End INV_IN.
 
 End Syntax.
-
-Module Atoms.
-
-  Local Set Printing Universes.
-
-  Local Notation index := nat.
-
-  Section ATOMS.
-
-    Polymorphic Inductive t :=
-      | own_unit (x : unit)
-      | owni (n : index) (i : positive) (p : @Syntax.t t)
-    .
-
-    Definition test1 n i :=
-      owni n i (Syntax.atom (owni n i (Syntax.empty))).
-    Definition test2 n i :=
-      owni n i (Syntax.and (Syntax.empty) (Syntax.pure (1 = 1))).
-    Fail Definition test3 n i :=
-      @Syntax.ex t _ (fun (s : @Syntax.t t) => Syntax.pure (s = Syntax.atom (owni n i (@Syntax.ex t _ (fun (s' : Syntax.t) => Syntax.pure (s' = Syntax.atom (owni n i Syntax.empty))))))).
-    TODO
-    Definition test4 n i :=
-      @Syntax.ex t _ (fun (s : Syntax.t) => Syntax.pure (s = Syntax.atom (owni n i (@Syntax.ex t _ (fun m => Syntax.and Syntax.empty (Syntax.pure (m = 1))))))).
-    Definition test3 n i :=
-      owni n i (Syntax.ex (fun (s : Syntax.t) => Syntax.empty)).
-    Definition test2 n i :=
-      owni n i (Syntax.ex (fun (s : Syntax.t) => Syntax.pure (s = Syntax.empty))).
-
-    (* Polymorphic Inductive t@{i j k} : Type@{k} := *)
-    (*   | own_unit (x : unit) *)
-    (*   | owni (n : index) (i : positive) (p : @Syntax.t@{i j} t) *)
-    (* . *)
-
-    (* Polymorphic Fixpoint embedT@{i j k l | k < l} (a : t@{i j k}) : t@{i j l} := *)
-    (*   match a with *)
-    (*   | owni n i (p : Syntax.t) => owni n i (Syntax.castA@{k l i j} embedT p) *)
-    (*   end. *)
-
-
-  (* Definition OwnE `{@GRA.inG (index ==> CoPset.t)%ra Σ} (n : index) (E : coPset) := *)
-  (*   OwnM (@maps_to_res index CoPset.t n (Some E)). *)
-
-  (* Definition OwnD `{@GRA.inG (index ==> Gset.t)%ra Σ} (n : index) (D : gset positive) := *)
-  (*   OwnM (@maps_to_res index Gset.t n (Some D)). *)
-
-  (* Definition OwnI_white {Var} (n : index) (i : positive) (p : Var) : IInvSetRA Var := *)
-  (*   @maps_to_res index (Auth.t (positive ==> URA.agree Var))%ra *)
-  (*                n (Auth.white (@maps_to_res positive (URA.agree Var) i (Some (Some p)))). *)
-
-  (* Definition OwnI {Var} `{@GRA.inG (IInvSetRA Var) Σ} (n : index) (i : positive) (p : Var) := *)
-  (*   OwnM (OwnI_white n i p). *)
-
-  (* Definition inv_auth_black (I : gmap positive Var) : IInvSetRA Var := *)
-  (*   @maps_to_res index _ *)
-  (*                n (@Auth.black (positive ==> URA.agree Var)%ra *)
-  (*                               (fun (i : positive) => Some <$> (I !! i))). *)
-
-  (* Definition inv_auth (I : gmap positive Var) := *)
-  (*   OwnM (inv_auth_black I). *)
-
-  (* Definition inv_satall (I : gmap positive Var) := *)
-  (*   ([∗ map] i ↦ p ∈ I, (prop p) ∗ OwnD n {[i]} ∨ OwnE n {[i]})%I. *)
-
-  (* Definition wsat : iProp := (∃ I, inv_auth I ∗ inv_satall I)%I. *)
-
-  (* Definition inv (N : namespace) P := *)
-  (*   (∃ p, ∃ i, ⌜prop p = P⌝ ∧ ⌜i ∈ (↑N : coPset)⌝ ∧ OwnI n i p)%I. *)
-
-  (* Definition FUpd (A : iProp) (E1 E2 : coPset) (P : iProp) : iProp := *)
-  (*   A ∗ wsat n ∗ OwnE n E1 -∗ #=> (A ∗ wsat n ∗ OwnE n E2 ∗ P). *)
-
-  End ATOMS.
-
-  Section INTERP.
-
-    Context `{Σ : GRA.t}.
-    Context `{@GRA.inG Unit Σ}.
-
-    Definition to_semantics (a : t) : iProp :=
-      match a with
-      | own_unit x => OwnM (x : Unit)
-      end.
-
-  End INTERP.
-
-  Section INVSET.
-
-    Context `{Σ : GRA.t}.
-    Context `{@GRA.inG Unit Σ}.
-
-    Global Instance I : @InvSet Σ t :=
-      {| prop := to_semantics |}.
-
-  End INVSET.
-
-End Atoms.
-
-Section TEST.
-
-  Local Notation index := nat.
-
-  Local Set Printing Universes.
-
-  Context `{Σ : GRA.t}.
-  Context `{A : Type}.
-  Context `{Atomics : @InvSet Σ A}.
-  Context `{@GRA.inG (IInvSetRA (@t A)) Σ}.
-
-  Print Universes.
-
-  Definition inv_test (n : nat) (i : positive) (P : iProp) : Syntax.t :=
-    Syntax.ex (fun (p : Syntax.t) =>
-                 (Syntax.and
-                   (Syntax.pure (@prop _ _ (@Syntax.I _ _ Atomics _) p = P))
-                   (Syntax.owni n i p))).
-Syntax.I@{} = 
-λ (Σ : GRA.t) (A : Type@{Fairness.LogicSyntaxUP.597}) (Atomics : InvSet A) 
-  (H : GRA.inG (IInvSetRA Syntax.t@{Fairness.LogicSyntaxUP.598 Fairness.LogicSyntaxUP.599}) Σ),
-  {| prop := Syntax.to_semantics |}
-     : ∀ (Σ : GRA.t) (A : Type@{Fairness.LogicSyntaxUP.597}),
-         InvSet A
-         → GRA.inG (IInvSetRA Syntax.t@{Fairness.LogicSyntaxUP.598 Fairness.LogicSyntaxUP.599}) Σ
-           → InvSet Syntax.t@{Fairness.LogicSyntaxUP.589 Fairness.LogicSyntaxUP.590}
-(*  |= Set < InvSet.u0
-       Set < OwnI.u0
-       Fairness.LogicSyntaxUP.589 < InvSet.u0
-       Fairness.LogicSyntaxUP.589 < OwnI.u0
-       Fairness.LogicSyntaxUP.590 < InvSet.u0
-       Fairness.LogicSyntaxUP.590 < OwnI.u0
-       Fairness.LogicSyntaxUP.396 <= InvSet.u0
-       Fairness.LogicSyntaxUP.396 <= OwnI.u0
-       Fairness.LogicSyntaxUP.588 <= InvSet.u0
-       Fairness.LogicSyntaxUP.588 <= Fairness.LogicSyntaxUP.396
-       Fairness.LogicSyntaxUP.589 <= Univ_obligation_1.u0
-       Fairness.LogicSyntaxUP.590 <= Ex_obligation_1.u0
-       Fairness.LogicSyntaxUP.597 <= Fairness.LogicSyntaxUP.396
-       Fairness.LogicSyntaxUP.597 <= Fairness.LogicSyntaxUP.588
-       Fairness.LogicSyntaxUP.589 = Fairness.LogicSyntaxUP.598
-       Fairness.LogicSyntaxUP.590 = Fairness.LogicSyntaxUP.599 *)
-  Definition inv (N : namespace) P :=
-    (∃ p, ∃ i, ⌜prop p = P⌝ ∧ ⌜i ∈ (↑N : coPset)⌝ ∧ OwnI n i p)%I.
-
-  Definition form1 : @Syntax.it A 3 :=
-    @Syntax.ex _ (@Syntax.it A 2) (fun s => Syntax.pure (@prop _ _ (@Syntax.I _ _ Atomics 2) s = (⌜True⌝ ∗ ⌜False⌝)%I)).
-
-  (* Compute @prop _ _ (@Syntax.I _ _ Atomics 3) form1. *)
-
-  Lemma test1 :
-    @prop _ _ (@Syntax.I _ _ Atomics 3) form1 =
-      (∃ (s : @Syntax.it A 2), ⌜(@prop _ _ (@Syntax.I _ _ Atomics 2) s = (⌜True⌝ ∗ ⌜False⌝)%I)⌝)%I.
-  Proof.
-    ss.
-  Qed.
-
-  Definition form1' : @Syntax.it A 3 :=
-    Syntax.ex (fun (s : @Syntax.it A 2) => Syntax.pure (prop (InvSet:=Syntax.I) s = (⌜True⌝ ∗ ⌜False⌝)%I)).
-
-  Set Printing All.
-  Print form1'.
-  Unset Printing All.
-
-  (* Local Notation it n := (@Syntax.it A n). *)
-
-  (* Definition form1'' : it 3 := *)
-  (*   Syntax.ex (fun (s : it 2) => Syntax.pure (prop (InvSet:=Syntax.I) s = (⌜True⌝ ∗ ⌜False⌝)%I)). *)
-
-End TEST.
-
-Section INDEXEDINV.
-
-  Context `{Σ : GRA.t}.
-  Context `{A : Type}.
-  Context `{Atomics : @InvSet Σ A}.
-
-  Fixpoint indexed (n : nat) (BaseI : @InvSet Σ (@Syntax.t A)) : @InvSet Σ (@Syntax.t A) :=
-    match n with
-      | O => @Syntax.I Σ A Atomics 
-
-
-End INDEXEDINV.
-
-
-
-Section TEST.
-
-  Local Notation index := nat.
-
-  Context `{Σ : GRA.t}.
-  Context `{A : Type}.
-  Context `{Atomics : @InvSet Σ A}.
-
-  Definition form1 : @Syntax.it A 3 :=
-    @Syntax.ex _ (@Syntax.it A 2) (fun s => Syntax.pure (@prop _ _ (@Syntax.I _ _ Atomics 2) s = (⌜True⌝ ∗ ⌜False⌝)%I)).
-
-  (* Compute @prop _ _ (@Syntax.I _ _ Atomics 3) form1. *)
-
-  Lemma test1 :
-    @prop _ _ (@Syntax.I _ _ Atomics 3) form1 =
-      (∃ (s : @Syntax.it A 2), ⌜(@prop _ _ (@Syntax.I _ _ Atomics 2) s = (⌜True⌝ ∗ ⌜False⌝)%I)⌝)%I.
-  Proof.
-    ss.
-  Qed.
-
-  Definition form1' : @Syntax.it A 3 :=
-    Syntax.ex (fun (s : @Syntax.it A 2) => Syntax.pure (prop (InvSet:=Syntax.I) s = (⌜True⌝ ∗ ⌜False⌝)%I)).
-
-  Set Printing All.
-  Print form1'.
-  Unset Printing All.
-
-  (* Local Notation it n := (@Syntax.it A n). *)
-
-  (* Definition form1'' : it 3 := *)
-  (*   Syntax.ex (fun (s : it 2) => Syntax.pure (prop (InvSet:=Syntax.I) s = (⌜True⌝ ∗ ⌜False⌝)%I)). *)
-
-  Local Set Printing Universes.
-
-  Definition iisra0 := IInvSetRA (@Syntax.it A 0).
-  Definition iisra1 := IInvSetRA (@Syntax.it A 1).
-  (* Definition iisra n := IInvSetRA (@Syntax.it A n). *)
-  Definition iisra := IInvSetRA (@Syntax.t A).
-
-  Definition OwnI_white_test (i : positive) (p : @Syntax.t A) : IInvSetRA (@Syntax.t A) :=
-    @maps_to_res index (Auth.t (positive ==> URA.agree (@Syntax.t A)))%ra
-                 2
-                 (Auth.white (@maps_to_res positive (URA.agree (@Syntax.t A))
-                                           i (Some (Some (Syntax.ex (fun s => Syntax.pure (s = p))))))).
-
-  Definition OwnI_test `{Σ0 : GRA.t} `{@GRA.inG (IInvSetRA (@Syntax.t A)) Σ0}
-             (i : positive) (p : @Syntax.t A) :=
-    OwnM (OwnI_white_test i p).
-
-  Definition OwnI_white_test2 (i : positive) (p : @Syntax.t A) : IInvSetRA (@Syntax.t A) :=
-    @maps_to_res index (Auth.t (positive ==> URA.agree (@Syntax.t A)))%ra
-                 2
-                 (Auth.white (@maps_to_res positive (URA.agree (@Syntax.t A))
-                                           i (Some (Some (Syntax.ex (fun s => Syntax.pure (s = p))))))).
-
-  Definition OwnI_test2 `{Σ0 : GRA.t} `{@GRA.inG (IInvSetRA (@Syntax.t A)) Σ0}
-             (i : positive) (p : @Syntax.t A) :=
-    OwnM (OwnI_white_test2 i p).
-
-  Definition OwnI_test3 `{Σ0 : GRA.t} `{@GRA.inG (IInvSetRA (@Syntax.t A)) Σ0}
-             (i : positive) (p : @Syntax.t A) (q : @Syntax.t A) :=
-    ((OwnI_test i p) ∗ (OwnI_test2 i q))%I.
-
-  Print Universes.
-OwnI_test3 = 
-λ (Σ0 : GRA.t) (H : GRA.inG (IInvSetRA Syntax.t@{OwnI_white_test.u2 OwnI_white_test.u3}) Σ0) 
-  (i : positive) (p : Syntax.t@{OwnI_white_test.u0 OwnI_white_test.u1}) 
-  (q : Syntax.t@{OwnI_white_test2.u0 OwnI_white_test2.u1}), OwnI_test i p ** OwnI_test2 i q
-     : ∀ Σ0 : GRA.t,
-         GRA.inG (IInvSetRA Syntax.t@{OwnI_white_test.u2 OwnI_white_test.u3}) Σ0
-         → positive
-           → Syntax.t@{OwnI_white_test.u0 OwnI_white_test.u1}
-             → Syntax.t@{OwnI_white_test2.u0 OwnI_white_test2.u1} → iProp
-(* iisra.u0 < IInvSetRA.u0 *)
-(* iisra.u1 < IInvSetRA.u0 *)
-OwnI_white_test = 
-λ (i : positive) (p : Syntax.t@{OwnI_white_test.u0 OwnI_white_test.u1}),
-  maps_to_res 2
-    (Auth.white
-       (maps_to_res i
-          (Some
-             (Some
-                (Syntax.ex@{OwnI_white_test.u2 OwnI_white_test.u3}
-                   (λ s : Syntax.t@{OwnI_white_test.u0 OwnI_white_test.u1},
-                      Syntax.pure@{OwnI_white_test.u2 OwnI_white_test.u3} (s = p)))))))
-     : positive
-       → Syntax.t@{OwnI_white_test.u0 OwnI_white_test.u1}
-         → IInvSetRA Syntax.t@{OwnI_white_test.u2 OwnI_white_test.u3}
-OwnI_white_test.u0 < Coq.Relations.Relation_Definitions.1
-                   < OwnI_white_test.u3
-OwnI_white_test.u1 < Coq.Relations.Relation_Definitions.1
-                   < OwnI_white_test.u3
-OwnI_white_test.u2 < IInvSetRA.u0
-                   < MRet.u0
-                   < URA.agree_obligation_4.u0
-OwnI_white_test.u3 < IInvSetRA.u0
-                   < MRet.u0
-                   < URA.agree_obligation_4.u0
-
-OwnI_test = 
-λ (Σ0 : GRA.t) (H : GRA.inG (IInvSetRA Syntax.t@{OwnI_white_test.u2 OwnI_white_test.u3}) Σ0) 
-  (i : positive) (p : Syntax.t@{OwnI_white_test.u0 OwnI_white_test.u1}),
-  OwnM (OwnI_white_test i p)
-     : ∀ Σ0 : GRA.t,
-         GRA.inG (IInvSetRA Syntax.t@{OwnI_white_test.u2 OwnI_white_test.u3}) Σ0
-         → positive → Syntax.t@{OwnI_white_test.u0 OwnI_white_test.u1} → iProp
-
-  Definition cast (A : Type) : nat -> A
-
-  Goal @Syntax.it A 2 = @Syntax.it A 3.
-  Proof.
-    ss.
-  Qed.
-
-  Lemma test_up_type : forall n m, @Syntax.it A n = @Syntax.it A m.
-  Proof.
-    ss.
-  Qed.
-
-  (* Print Universes. *)
-(* test_up_type.u0 < test_up_type.u2 *)
-(* test_up_type.u1 < test_up_type.u2 *)
-(* test_up_type.u2 < Coq.Relations.Relation_Definitions.1 *)
-(* test_up_type.u3 = test_up_type.u0 *)
-(* test_up_type.u4 = test_up_type.u1 *)
-
-  (* Goal @Syntax.it (@Syntax.it A 1) 2 = @Syntax.it A 3. *)
-  (* Proof. *)
-  (*   ss. *)
-  (* Abort. *)
-
-  (* Goal @Syntax.it nat 2 = @Syntax.it unit 2. *)
-  (* Proof. *)
-  (*   ss. *)
-  (* Abort. *)
-
-  TODO
-
-  Definition inv (N : namespace) P :=
-    (∃ p, ∃ i, ⌜prop p = P⌝ ∧ ⌜i ∈ (↑N : coPset)⌝ ∧ OwnI n i p)%I.
-
-  (* Fixpoint IndexedSyntax (n : nat) : Type := *)
-  (*   match n with *)
-  (*   | O => (@Syntax.t A) *)
-  (*   | S n' => (@Syntax.t (IndexedSyntax n')) *)
-  (*   end. *)
-
-  (* Fixpoint indexed (n : index) : InvSet (IndexedSyntax n) := *)
-  (*   match n with *)
-  (*   | O => {| prop := @Syntax.to_semantics _ A Atomics |} *)
-  (*   | S n' => {| prop := @Syntax.to_semantics _ (IndexedSyntax n') (indexed n') |} *)
-  (*   end. *)
-
-
-  Local Instance Σ: GRA.t:=
-    GRA.of_list [].
-
-  Local Instance Atomics : InvSet unit :=
-    {| prop := fun _ => emp%I |}.
-
-
-  Lemma test0 :
-    forall (n : nat),
-      @prop _ _ (Syntax.InvSet) (Syntax.pure (@prop _ _ Syntax.InvSet (Syntax.sepconj (Syntax.pure True) (Syntax.atom tt)) = (⌜True⌝ ∗ emp)%I))
-      =
-        (⌜(@prop _ _ (Syntax.InvSet) (Syntax.sepconj (Syntax.pure True) (Syntax.atom tt)) = (⌜True⌝ ∗ emp)%I)⌝)%I.
-  Proof.
-    i. ss.
-  Qed.
-
-  Definition inv (N : namespace) P :=
-    (∃ p, ∃ i, ⌜prop p = P⌝ ∧ ⌜i ∈ (↑N : coPset)⌝ ∧ OwnI n i p)%I.
-
-  Lemma test1 :
-    forall (n : nat),
-      @prop _ _ (SynInvs (S n)) (Syntax.pure (@prop _ _ (SynInvs n) (Syntax.sepconj (Syntax.pure True) (Syntax.pure False)) = (⌜True⌝ ∗ ⌜False⌝)%I))
-      =
-        (⌜(@prop _ _ (SynInvs n) (Syntax.sepconj (Syntax.pure True) (Syntax.pure False)) = (⌜True⌝ ∗ ⌜False⌝)%I)⌝)%I.
-  Proof.
-    i. ss.
-  Qed.
-
-  Lemma test2 :
-    forall (n : nat),
-      @prop _ _ (SynInvs (n)) (Syntax.pure (@prop _ _ (SynInvs n) (Syntax.sepconj (Syntax.pure True) (Syntax.pure False)) = (⌜True⌝ ∗ ⌜False⌝)%I))
-      =
-        (⌜(@prop _ _ (SynInvs n) (Syntax.sepconj (Syntax.pure True) (Syntax.pure False)) = (⌜True⌝ ∗ ⌜False⌝)%I)⌝)%I.
-  Proof.
-    i. ss.
-  Qed.
-
-End TEST.
