src/tlogic/TemporalLogic.v
@@ -1,0 +1,305 @@
+From stdpp Require Import coPset gmap namespaces.
+From sflib Require Import sflib.
+From Fairness Require Import PCM IProp IPM.
+From Fairness Require Import IndexedInvariants LogicSyntaxHOAS.
+From iris Require Import bi.big_op.
+From iris Require base_logic.lib.invariants.
+
+Local Notation index := nat.
+
+Module Base.
+
+  Inductive t : Type :=
+  | unitT
+  | natT
+  | boolT
+  | positiveT
+  | QpT
+  | coPsetT
+  | gsetT (K : Type) {EqDec : EqDecision K} {Cnt : Countable K}.
+
+  Definition sem (ty : t) : Type :=
+    match ty with
+    | unitT => unit
+    | natT => nat
+    | boolT => bool
+    | positiveT => positive
+    | QpT => Qp
+    | coPsetT => coPset
+    | gsetT K => gset K
+    end.
+
+End Base.
+
+Module Atoms.
+
+  Section ATOMS.
+
+    Context `{T : Type}.
+
+    TODO: more atoms
+
+    (* Atoms do not interpret arguments. *)
+    Inductive t {Typ : @Syntax.type T -> Type} : Type :=
+      | owni (n : index) (i : positive) (p : @Syntax.t T Typ (@t Typ))
+    .
+
+  End ATOMS.
+
+  Section INTERP.
+
+    Context `{Σ : GRA.t}.
+    Context `{T : Type}.
+    Context `{TSem : T -> Type}.
+    (* Context `{As : (@type T -> Type) -> Type}. *)
+
+    Local Notation typing := (@Syntax.Typ T TSem (@t T)).
+    Local Notation As := (fun (i : index) => @t T (typing i)).
+    Local Notation Formulas := (fun (i : index) => @Syntax.t T (typing i) (As i)).
+
+    (* Context `{Atoms : @IInvSet Σ (fun (n : index) => As (typing n))}. *)
+
+    (* Set Printing Universes. *)
+    (* Print Universes. *)
+
+    (* Context `{@GRA.inG (IInvSetRA As) Σ}. *)
+    Context `{@GRA.inG (IInvSetRA Formulas) Σ}.
+
+    Definition indexed_iProp (n : index) (P : iProp) : index -> iProp :=
+      fun m => match PeanoNat.Nat.eqb_spec m n with
+            | ReflectT _ _ => P
+            | ReflectF _ _ => ⌜False⌝%I
+            end.
+
+    Definition to_semantics (n : index) (a : @t T (typing n)) : iProp :=
+      match a with
+      | owni m i p => indexed_iProp n (@OwnI Σ Formulas _ n i p) m
+      end.
+
+  End INTERP.
+
+  (*   Definition OwnE `{@GRA.inG (index ==> CoPset.t)%ra Σ} (n : index) (E : coPset) := *)
+  (*   OwnM (@maps_to_res index CoPset.t n (Some E)). *)
+
+  (* Definition OwnD `{@GRA.inG (index ==> Gset.t)%ra Σ} (n : index) (D : gset positive) := *)
+  (*   OwnM (@maps_to_res index Gset.t n (Some D)). *)
+
+  Definition OwnI_white {Vars} (n : index) (i : positive) (p : Vars n) : IInvSetRA Vars :=
+    @maps_to_res_dep index (@InvSetRA Vars)
+                     n
+                     (Auth.white (@maps_to_res positive (URA.agree (Vars n)) i (Some (Some p)))).
+
+  Definition OwnI {Vars} `{@GRA.inG (IInvSetRA Vars) Σ} (n : index) (i : positive) (p : Vars n) :=
+    OwnM (OwnI_white n i p).
+
+  (* Definition inv_auth_black (I : gmap positive Var) : IInvSetRA Vars := *)
+  (*   @maps_to_res_dep index _ *)
+  (*                    n (@Auth.black (positive ==> URA.agree Var)%ra *)
+  (*                                   (fun (i : positive) => Some <$> (I !! i))). *)
+
+  (* Definition inv_auth (I : gmap positive Var) := *)
+  (*   OwnM (inv_auth_black I). *)
+
+  (* Definition inv_satall (I : gmap positive Var) := *)
+  (*   ([∗ map] i ↦ p ∈ I, (prop n p) ∗ OwnD n {[i]} ∨ OwnE n {[i]})%I. *)
+
+  (* Definition wsat : iProp := (∃ I, inv_auth I ∗ inv_satall I)%I. *)
+
+  (* Definition inv (N : namespace) P := *)
+  (*   (∃ p, ∃ i, ⌜prop n p = P⌝ ∧ ⌜i ∈ (↑N : coPset)⌝ ∧ OwnI n i p)%I. *)
+
+  (* Definition FUpd (A : iProp) (E1 E2 : coPset) (P : iProp) : iProp := *)
+  (*   A ∗ wsat n ∗ OwnE n E1 -∗ #=> (A ∗ wsat n ∗ OwnE n E2 ∗ P). *)
+
+  Section TEST.
+
+    Import Syntax.
+
+    Context `{TSem : T -> Type}.
+
+    Local Notation t := Atoms.t.
+
+
+    Local Notation typing := (@Syntax.Typ T TSem t).
+    Local Notation Formulas := (fun (i : index) => @Syntax.t T (typing i) (t (typing i))).
+
+    Definition test1 : Formulas 3 :=
+      atom (owni 4 xH (atom (owni 2 xH empty))).
+
+    Definition test_OwnI (n : index) (i : positive) (p : Formulas n) : t (typing n) :=
+      @owni (typing n) n i p.
+
+    (* Set Printing All. *)
+
+  End TEST.
+
+End Atoms.
+
+
+
+(*   Context `{T : Type}. *)
+(*     Context `{TSem : T -> Type}. *)
+
+(*     (* Atoms should not interpret arguments. *) *)
+(*     Inductive As (V : @type T -> Type) : Type := *)
+(*       | owni (p : V formulaT) *)
+(*     . *)
+(*     (* Inductive As (V : @type T -> Type) : Type := *) *)
+(*     (*   | owni (i : index) (p : @t T V (As V)) *) *)
+(*     (* . *) *)
+
+(*     Definition typing (i : index) : @type T -> Type := *)
+(*       @Typ T TSem As i. *)
+
+(*     (* Definition ttt1 : As (typing 2) := owni (typing 2) 0 (ex formulaT (fun s => pure (s = empty))). *) *)
+(*     (* Compute ttt1. *) *)
+(*     Definition ttt1 : As (typing 2) := owni (typing 2) (ex formulaT (fun s => pure (s = empty))). *)
+(*     Compute ttt1. *)
+(*     Goal typing 2 formulaT = @t T (typing 1) (As (typing 1)). *)
+(*     Proof. *)
+(*       ss. *)
+(*     Qed. *)
+
+(*     Definition inv (i : index) (p : typing i formulaT) : *)
+(*       @t T (typing i) (As (typing i)) := *)
+(*       atom (owni _ p). *)
+(*     (* Definition inv (n i : index) (p : @t T (typing i) (As (typing i))) : *) *)
+(*     (*   @t T (typing i) (As (typing i)) := *) *)
+(*     (*   atom (owni _ n p). *) *)
+(*     Definition wsat (i : index) : *)
+(*       @t T (typing i) (As (typing i)) := *)
+(*       ex formulaT (fun (p : typing i formulaT) => sepconj (lift p) (inv i p)). *)
+
+(*     (* Definition inv0 (n i : index) (p : @t T (typing 2) (As (typing 2))) : *) *)
+(*     (*   @t T (typing 3) (As (typing 2)) := *) *)
+(*     (*   atom (owni _ n p). *) *)
+
+(*     (* (* Definition of As enforces that  *) *)
+(*     (*    p should have the same typing level for itself and its atom  *) *)
+(*     (*  *) *) *)
+(*     (* Fail Definition inv1 (n : index) (p : @t T (typing 2) (As (typing 3))) : *) *)
+(*     (*   @t T (typing 2) (As (typing 3)) := *) *)
+(*     (*   atom (owni _ n p). *) *)
+
+(*     (* Definition inv2 q := *) *)
+(*     (*   inv 0 3 (atom (owni _ 1 (atom (owni _ 2 q)))). *) *)
+
+(*     (* Fail Definition inv2' q := *) *)
+(*     (*   inv 0 3 (atom (owni _ 1 (atom (owni (typing 2) 2 q)))). *) *)
+
+(*     (* Set Printing All. *) *)
+
+(*     (* Definition inv (N : namespace) P := *) *)
+(*     (*   (∃ p, ∃ i, ⌜prop p = P⌝ ∧ ⌜i ∈ (↑N : coPset)⌝ ∧ OwnI n i p)%I. *) *)
+
+
+
+
+
+(*   Section TEST. *)
+
+(*     Context `{A : Type}. *)
+
+(*     Variant tBase := | tBool | tNat. *)
+(*     Definition tBase_sem (b : tBase) : Type := *)
+(*       match b with | tBool => bool | tNat => nat end. *)
+
+(*     Let Var := @Var tBase tBase_sem A. *)
+
+(*     Compute Var 3 formulaT. *)
+
+(*     (* Goal Var 3 formulaT = @t _ (Var 2) A formulaT. *) *)
+(*     Goal Var 3 formulaT = @t _ (Var 2) A. *)
+(*     Proof. ss. Qed. *)
+
+(*     Definition syn_bad i := @t tBase (@Var i) A. *)
+(*     Notation syn i := (@t tBase (@Var i) A). *)
+
+(*     (* Definition form1 : @syn 2 formulaT := *) *)
+(*     Definition form1 : @syn 2 := *)
+(*       @ex _ _ _ (baseT tBool) (fun b => empty). *)
+
+(*     (* Goal (syn 1 formulaT) = (Var 2 formulaT). *) *)
+(*     Goal (syn 1) = (Var 2 formulaT). *)
+(*     Proof. ss. Qed. *)
+
+(*     (* Definition form2 : @syn 2 formulaT := *) *)
+(*       (* @ex _ _ _ formulaT (fun (s : Var 2 formulaT) => and (var _ s) (var _ s)). *) *)
+(*     Definition form2 : @syn 2 := *)
+(*       @ex _ _ _ formulaT (fun (s : Var 2 formulaT) => pure (s = impl empty empty)). *)
+
+(*     (* Definition form3 : @syn 2 formulaT := *) *)
+(*     (*   @ex _ _ _ formulaT (fun (s : @t tBase (Var 1) A formulaT) => and (var _ s) (var _ s)). *) *)
+(*     Definition form3 : @syn 2 := *)
+(*       @ex _ _ _ formulaT (fun (s : @t tBase (Var 1) A) => pure (s = impl empty empty)). *)
+
+(*     (* Definition form4 : @syn 2 formulaT := *) *)
+(*     (*   @ex _ _ _ formulaT (fun (s : @syn 1 formulaT) => and (var _ s) (var _ s)). *) *)
+(*     Definition form4 : @syn 2 := *)
+(*       @ex _ _ _ formulaT (fun (s : @syn 1) => pure (s = impl empty empty)). *)
+
+(*     (* Definition form5 : @syn 2 formulaT := *) *)
+(*     (*   @ex _ _ _ formulaT (fun (s : @syn 1 formulaT) => pure (s = wand empty empty)). *) *)
+(*     Definition form5 : @syn 2 := *)
+(*       @ex _ _ _ formulaT (fun (s : @syn 1) => pure (s = wand empty empty)). *)
+
+(*   End TEST. *)
+
+(* Section TEST. *)
+
+(*     Context `{T : Type}. *)
+(*     Context `{TSem : T -> Type}. *)
+
+(*     (* Atoms should not interpret arguments. *) *)
+(*     Inductive As (V : @type T -> Type) : Type := *)
+(*       | owni (p : V formulaT) *)
+(*     . *)
+(*     (* Inductive As (V : @type T -> Type) : Type := *) *)
+(*     (*   | owni (i : index) (p : @t T V (As V)) *) *)
+(*     (* . *) *)
+
+(*     Definition typing (i : index) : @type T -> Type := *)
+(*       @Typ T TSem As i. *)
+
+(*     (* Definition ttt1 : As (typing 2) := owni (typing 2) 0 (ex formulaT (fun s => pure (s = empty))). *) *)
+(*     (* Compute ttt1. *) *)
+(*     Definition ttt1 : As (typing 2) := owni (typing 2) (ex formulaT (fun s => pure (s = empty))). *)
+(*     Compute ttt1. *)
+(*     Goal typing 2 formulaT = @t T (typing 1) (As (typing 1)). *)
+(*     Proof. *)
+(*       ss. *)
+(*     Qed. *)
+
+(*     Definition inv (i : index) (p : typing i formulaT) : *)
+(*       @t T (typing i) (As (typing i)) := *)
+(*       atom (owni _ p). *)
+(*     (* Definition inv (n i : index) (p : @t T (typing i) (As (typing i))) : *) *)
+(*     (*   @t T (typing i) (As (typing i)) := *) *)
+(*     (*   atom (owni _ n p). *) *)
+(*     Definition wsat (i : index) : *)
+(*       @t T (typing i) (As (typing i)) := *)
+(*       ex formulaT (fun (p : typing i formulaT) => sepconj (lift p) (inv i p)). *)
+
+(*     (* Definition inv0 (n i : index) (p : @t T (typing 2) (As (typing 2))) : *) *)
+(*     (*   @t T (typing 3) (As (typing 2)) := *) *)
+(*     (*   atom (owni _ n p). *) *)
+
+(*     (* (* Definition of As enforces that  *) *)
+(*     (*    p should have the same typing level for itself and its atom  *) *)
+(*     (*  *) *) *)
+(*     (* Fail Definition inv1 (n : index) (p : @t T (typing 2) (As (typing 3))) : *) *)
+(*     (*   @t T (typing 2) (As (typing 3)) := *) *)
+(*     (*   atom (owni _ n p). *) *)
+
+(*     (* Definition inv2 q := *) *)
+(*     (*   inv 0 3 (atom (owni _ 1 (atom (owni _ 2 q)))). *) *)
+
+(*     (* Fail Definition inv2' q := *) *)
+(*     (*   inv 0 3 (atom (owni _ 1 (atom (owni (typing 2) 2 q)))). *) *)
+
+(*     (* Set Printing All. *) *)
+
+(*     (* Definition inv (N : namespace) P := *) *)
+(*     (*   (∃ p, ∃ i, ⌜prop p = P⌝ ∧ ⌜i ∈ (↑N : coPset)⌝ ∧ OwnI n i p)%I. *) *)
+
+(* End TEST. *)
